txn-data-consistency/EP+_Sorted.thy
@@ -1,15 +1,10 @@
 section \<open>EP+ Event System for well-sorted executions\<close>
 
 theory "EP+_Sorted"
-  imports "EP+"
+  imports "EP+" "EP+_Reduction"
 begin
 
 \<comment> \<open>Updated Events\<close>
-
-datatype 'v ev =
-  RInvoke cl_id "key set" | Read cl_id key 'v txid tstmp tstmp | RDone cl_id "key \<rightharpoonup> 'v" sqn view |
-  WInvoke cl_id "key \<rightharpoonup> 'v" | WCommit cl_id "key \<rightharpoonup> 'v" tstmp sqn view | WDone cl_id "key \<rightharpoonup> 'v" |
-  RegR key txid0 txid tstmp | PrepW key txid 'v | CommitW key txid 'v tstmp | Skip2
 
 definition read_done_G_s where
   "read_done_G_s cl kv_map sn u'' s \<equiv>
@@ -25,7 +20,7 @@ definition write_commit_G_s where
   "write_commit_G_s cl kv_map cts sn u'' s \<equiv>
     write_commit_G cl kv_map cts sn s \<and>
     u'' = view_of (cts_order s) (get_view s cl) \<and>
-    (\<forall>k \<in> dom kv_map. \<forall>t \<in> set (cts_order s k). (cts, cl) > unique_ts (wtxn_cts s) t)"
+    (\<forall>k\<comment>\<open>\<in> dom kv_map\<close>. \<forall>t \<in> set (cts_order s k). (cts, Suc cl) > unique_ts (wtxn_cts s) t)"
 
 definition write_commit_s :: "cl_id \<Rightarrow> (key \<rightharpoonup> 'v) \<Rightarrow> tstmp \<Rightarrow> sqn \<Rightarrow> view \<Rightarrow> ('v, 'm) global_conf_scheme \<Rightarrow> ('v, 'm) global_conf_scheme \<Rightarrow> bool" where
   "write_commit_s cl kv_map cts sn u'' s s' \<equiv>
@@ -47,8 +42,8 @@ fun state_trans :: "('v, 'm) global_conf_scheme \<Rightarrow> 'v ev \<Rightarrow
   "state_trans s (CommitW svr t v cts)      s' \<longleftrightarrow> commit_write svr t v cts s s'" |
   "state_trans s Skip2 s' \<longleftrightarrow> s' = s"
 
-definition tps :: "('v ev, 'v global_conf) ES" where
-  "tps \<equiv> \<lparr>
+definition tps_s :: "('v ev, 'v global_conf) ES" where
+  "tps_s \<equiv> \<lparr>
     init = (=) state_init,
     trans = state_trans
   \<rparr>"
@@ -72,9 +67,9 @@ lemmas tps_trans_defs = tps_trans_top_defs tps_trans_GU_defs
 
 lemmas tps_trans_all_defs = tps_trans_defs ext_corder_def
 
-lemmas tps_defs = tps_def state_init_def
+lemmas tps_s_defs = tps_s_def state_init_def
 
-lemma tps_trans [simp]: "trans tps = state_trans" by (simp add: tps_def)
+lemma tps_trans [simp]: "trans tps_s = state_trans" by (simp add: tps_s_def)
 
 
 subsection \<open>Simulation function\<close>
@@ -105,5 +100,149 @@ fun med :: "'v ev \<Rightarrow> 'v label" where
   "med (RDone cl kv_map sn u'') = ET cl sn u'' (read_only_fp kv_map)" |
   "med (WCommit cl kv_map _ sn u'') = ET cl sn u'' (write_only_fp kv_map)" |
   "med _ = ETSkip"
+
+subsection \<open>Reduction: reachable states equivalence\<close>
+
+subsubsection \<open>Invariants\<close>
+definition Wtxn_Cts_T0 where
+  "Wtxn_Cts_T0 s k \<longleftrightarrow> wtxn_cts s T0 = Some 0"
+
+lemmas Wtxn_Cts_T0I = Wtxn_Cts_T0_def[THEN iffD2, rule_format]
+lemmas Wtxn_Cts_T0E[elim] = Wtxn_Cts_T0_def[THEN iffD1, elim_format, rule_format]
+
+lemma reach_wtxn_cts_t0 [simp, dest]: "reach tps_s s \<Longrightarrow> Wtxn_Cts_T0 s k"
+proof(induction s rule: reach.induct)
+  case (reach_init s)
+  then show ?case
+    by (auto simp add: Wtxn_Cts_T0_def tps_s_defs)
+next
+  case (reach_trans s e s')
+  then show ?case
+    by (induction e) (auto simp add: Wtxn_Cts_T0_def tps_trans_defs)
+qed
+
+
+subsubsection \<open>Lemmas\<close>
+
+\<comment> \<open>tps_s \<longrightarrow> good execs\<close> 
+lemma tps_s_ev_sub_tps:
+  "tps_s: s\<midarrow>e\<rightarrow> s' \<Longrightarrow> tps: s\<midarrow>e\<rightarrow> s'"
+  by (induction e) (auto simp add: read_done_s_def read_done_def read_done_G_s_def
+      write_commit_s_def write_commit_def write_commit_G_s_def)
+
+lemma reach_good_state_f_None:
+  "\<lbrakk> tps_s: s \<midarrow>e\<rightarrow> s'; reach tps_s s; ev_cts e = None; reach_good_state tps ev_cts s \<rbrakk> \<Longrightarrow> 
+     reach_good_state tps ev_cts s'"
+  apply (auto simp add: reach_good_state_def valid_exec_def tps_def)
+  subgoal for efl
+  apply (intro exI[where x="efl @ [(s, e, s')]"], auto simp add: efrag_snoc_good)
+    using tps_s_ev_sub_tps vef_snoc by fastforce.
+
+lemma reach_good_state_f_Some:
+  "\<lbrakk> Exec_frag s0 efl s \<in> Good_wrt ev_cts; ev_cts e = Some (cts, Suc cl);
+     \<forall>i < length (trace_of_efrag (Exec_frag s0 efl s)). \<forall>cts' cl'.
+       ev_cts (trace_of_efrag (Exec_frag s0 efl s) ! i) = Some (cts', cl')
+        \<longrightarrow> (cts, Suc cl) > (cts', cl')\<rbrakk>
+    \<Longrightarrow> Exec_frag s0 (efl @ [(s, e, s')]) s' \<in> Good_wrt ev_cts"
+  apply (auto simp add: Good_wrt_def inverted_pairs_def trace_of_efrag_append nth_append)
+  by (metis less_antisym order.asym)
+
+\<comment> \<open>good execs \<longrightarrow> tps_s\<close>
+lemma tps_non_commit_ev_sub_tps_s:
+  "tps: s\<midarrow>e\<rightarrow> s' \<Longrightarrow> \<not>commit_ev e  \<Longrightarrow> tps_s: s\<midarrow>e\<rightarrow> s'"
+  by (induction e) (auto)
+
+lemma tps_RDone_sub_tps_s:
+  "tps: s\<midarrow>RDone cl kv_map sn u''\<rightarrow> s' \<Longrightarrow>
+   tps_s: s\<midarrow>RDone cl kv_map sn (view_of (cts_order s) (get_view s cl))\<rightarrow> s'"
+  by (simp add: read_done_def read_done_s_def read_done_G_s_def)
+
+lemma lowest_ts_lt_all: "(0, 0) < (x :: nat, Suc y)" by (auto simp add: less_prod_def)
+
+lemma efrag_snoc_good_def:
+  "Exec_frag state_init (efl @ [(s, e, s')]) s' \<in> Good_wrt ev_cts \<longleftrightarrow>
+    (\<forall>j i. j < Suc (length (trace_of_efrag (Exec_frag state_init efl s))) \<longrightarrow> i < j \<longrightarrow>
+     (\<forall>cts cl. ev_cts ((trace_of_efrag (Exec_frag state_init efl s) @ [e]) ! j) = Some (cts, cl) \<longrightarrow>
+     (\<forall>cts' cl'. ev_cts (trace_of_efrag (Exec_frag state_init efl s) ! i) = Some (cts', cl') \<longrightarrow>
+           \<not> (cts, cl) < (cts', cl'))))"
+  by (auto simp add: Good_wrt_def inverted_pairs_def trace_of_efrag_append nth_append)
+
+lemma new_wrc_no_conflict:
+  "\<lbrakk> Exec_frag state_init (efl @ [(s, e, s')]) s' \<in> Good_wrt ev_cts;
+     ev_cts e = Some (cts, cl);
+     i < length efl;
+     ev_cts (trace_of_efrag (Exec_frag state_init efl s) ! i) = Some (cts', cl') \<rbrakk>
+     \<Longrightarrow> (cts, cl) \<ge> (cts', cl')"
+  unfolding efrag_snoc_good_def
+  by (metis lessI linorder_le_less_linear nth_append_length trace_of_efrag_length)
+
+lemma tps_WCommit_sub_tps_s:
+  "\<lbrakk> tps: s\<midarrow>WCommit cl kv_map cts sn u''\<rightarrow> s';
+     reach tps_s s;
+     valid_exec_frag tps (Exec_frag s0 efl s);
+     Exec_frag s0 (efl @ [(s, e, s')]) s' \<in> Good_wrt ev_cts\<rbrakk>
+    \<Longrightarrow> tps_s: s\<midarrow>WCommit cl kv_map cts sn (view_of (cts_order s) (get_view s cl))\<rightarrow> s'"
+    using Wtxn_Cts_T0_def[of s]
+    apply (auto simp add: write_commit_s_def write_commit_def write_commit_G_s_def unique_ts_def
+             lowest_ts_lt_all)
+    sorry
+
+lemma reach_tps_s_non_commit:
+  "\<lbrakk> tps: s \<midarrow>e\<rightarrow> s';
+    \<not>commit_ev e;
+    \<lbrakk> init tps s0; Exec_frag s0 efl s \<in> Good_wrt ev_cts \<rbrakk> \<Longrightarrow> reach tps_s s;
+    Exec_frag s0 (efl @ [(s, e, s')]) s' \<in> Good_wrt ev_cts;
+    init tps s0\<rbrakk>
+    \<Longrightarrow> reach tps_s s'"
+  by (metis tps_non_commit_ev_sub_tps_s efrag_trim_good reach_trans)
+
+
+subsubsection \<open>Proof reach tps_s = reach E\<close>
+
+lemma "reach tps_s s \<longleftrightarrow> reach_good_state tps ev_cts s"
+  unfolding reach_good_state_def valid_exec_def
+proof (intro iffI; clarsimp simp only: exec_frag.sel)
+  assume \<open>reach tps_s s\<close>
+  then show \<open>\<exists>s0 efl. (valid_exec_frag tps (Exec_frag s0 efl s) \<and> init tps s0) \<and> Exec_frag s0 efl s \<in> Good_wrt ev_cts\<close>
+  proof (induction rule: reach.induct)
+    case (reach_init s)
+    then show ?case
+      by (auto simp add: reach_good_state_def valid_exec_def tps_s_def tps_def Good_wrt_def
+          trace_of_efrag_def inverted_pairs_def)
+  next
+    case (reach_trans s e s')
+    then show ?case using reach_good_state_f_None[of s e s']
+      unfolding reach_good_state_def valid_exec_def
+    proof (induction e)
+      case (WCommit x1 x2 x3 x4 x5)
+      then show ?case apply (auto simp add: tps_def)
+        subgoal for efl
+        apply (intro exI[where x="efl @ [(s, WCommit x1 x2 x3 x4 x5, s')]"], auto)
+           apply (metis WCommit.prems(1) tps_def tps_s_ev_sub_tps vef_snoc)
+          apply (auto dest!: reach_good_state_f_Some[of _ efl])
+          apply (thin_tac "Exec_frag _ _ _ \<notin> _ _")
+          apply (simp add: Good_wrt_def inverted_pairs_def trace_of_efrag_append write_commit_s_def
+              write_commit_G_s_def unique_ts_def) sorry.
+
+      thm trace.induct
+
+    qed auto
+  qed
+next
+  fix s0 efl
+  assume a: \<open>valid_exec_frag tps (Exec_frag s0 efl s)\<close> \<open>init tps s0\<close> \<open>Exec_frag s0 efl s \<in> Good_wrt ev_cts\<close>
+  then show \<open>reach tps_s s\<close>
+  proof (induction "(Exec_frag s0 efl s)" arbitrary: efl s rule: valid_exec_frag.induct)
+    case (vef_snoc efl s e s')
+    then show ?case using reach_tps_s_non_commit[of s e s']
+    proof (induction e)
+      case (RDone x1 x2 x3 x4)
+      then show ?case by (metis tps_RDone_sub_tps_s efrag_trim_good reach_trans)
+    next
+      case (WCommit x1 x2 x3 x4 x5)
+      then show ?case by (metis tps_WCommit_sub_tps_s efrag_trim_good reach_trans)
+    qed auto
+  qed (auto simp add: tps_s_def tps_def)
+qed
 
 end
